Begin the fwd_det proof without arrays.

Janus.v
@@ -293,23 +293,28 @@ Section Janus.
 
   Inductive fwd_det G m s m' : Stmt_eval G m s m' -> Prop :=
     | stmt_fwd: forall se,
-         forall m'',
            bwd_det G m s m' se ->
            Stmt_eval G m s m' ->
-           Stmt_eval G m s m'' -> m' = m'' ->
            fwd_det G m s m' se
 
   with bwd_det G m s m' : Stmt_eval G m s m' -> Prop :=
     | stmt_bwd: forall se,
-      forall m'',
         fwd_det G m s m' se ->
-        Stmt_eval G m' s m ->
-        Stmt_eval G m'' s m -> m' = m'' ->
+        Stmt_eval G m s m' ->
         bwd_det G m s m' se.
 
   Scheme fwd_det_ind_2 := Induction for fwd_det Sort Prop
   with   bwd_det_ind_2 := Induction for bwd_det Sort Prop.
 
+  Check fwd_det_ind_2.
+
+  Definition fwd_stmt_det G m s m' (s0: Stmt_eval G m s m')
+    : fwd_det G m s m' s0 -> Prop :=
+    fun se => forall m'', Stmt_eval G m s m'' -> m' = m''.
+
+  Definition bwd_stmt_det G m s m' (s0: Stmt_eval G m s m')
+    : bwd_det G m s m' s0 -> Prop :=
+    fun se => forall m'', Stmt_eval G m'' s m' -> m = m''.
 
   Definition stmt_det G m s m' : Stmt_eval G m s m' -> Prop :=
     fun se => forall m'', Stmt_eval G m s m'' -> m' = m''.
@@ -319,6 +324,37 @@ Section Janus.
     fun le => forall m'',
       Stmt_loop_eval G m e1 s1 s2 e2 m'' -> m' = m''.
 
+  Theorem fwd_determinism: forall G m s m',
+    forall se,
+    fwd_det G m s m' se -> forall m'', Stmt_eval G m s m'' -> m' = m''.
+  Proof.
+    intros until m'.
+    apply
+      (fwd_det_ind_2 G m s m'
+        (fwd_stmt_det G m s m')
+        (bwd_stmt_det G m s m')); unfold fwd_stmt_det; intros.
+    generalize G m s m' s0 m'' H0.
+    apply (stmt_eval_ind_2
+      stmt_det
+      (fun G m e1 s1 s2 e2 m' =>
+        fun le => forall m'',
+          Stmt_loop_eval G m e1 s1 s2 e2 m'' -> m' = m''));
+    unfold stmt_det; intros; try (inversion H1; intuition); intros.
+
+    inversion H3; intuition.
+    inversion H2; [intuition | congruence].
+    inversion H2; [congruence | intuition].
+    inversion H2; intuition.
+
+    assert (m'0 = m'1). intuition. subst. congruence.
+    inversion H3. assert (m'0 = m''1). intuition. subst. congruence.
+    assert (m'0 = m'1). intuition. intuition. subst. intuition.
+
+    inversion H2; intuition.
+    inversion H2. unfold bwd_stmt_det in H. grind.
+    Abort.
+
+  (* This only works for no UNCALL *)
   Lemma Stmt_eval_det : forall G m s m',
     Stmt_eval G m s m' -> forall m'',
       Stmt_eval G m s m'' -> m' = m''.
